Simplified the core implementation of B* and changed its interface with binder macros, making them more flexible and forcing them to do more of the work.  In particular, there are no more special suffixes such as + and @ for binder names that change the way the core deals with them.  For every binder FOO,
(b* (((foo a b c) (asdf x y))) bla)

expands to

(patbind-FOO (a b c) ((asdf x y)) bla)

This means that the definition of the macro PATBIND-FOO may need to do
more work, such as binding (asdf x y) to a variable so that it won't be
evaluated more than once; but it has the flexibility to not do that if
that is appropriate, which was a problem in the old design.

Finally, symbol packages are now respected when constructing the
patbind- macro calls.  Whatever FOO's package is above is also the
package of PATBIND-FOO.

books/tools/bstar.lisp
@@ -69,14 +69,18 @@ support more binding constructs.
 Its syntax is
 (b* <list-of-bindings> . <list-of-result-forms>)
 where a result form is any ACL2 term, and a binding is
-(<binder-form> <expression>).  See below for discussion of binder forms.
+(<binder-form> [<expression>]).  See below for discussion of binder forms.
+Depending on the binder form, it may be that multiple expressions are allowed
+or only a single one.
 
+B* expands to multiple nestings of another macro PATBIND, analogously to how
+LET* expands to multiple nestings of LET.
 
 -- Basic let*-like usage --
 B* can be used exactly like LET*, except that it does not yet support DECLARE
 forms.  However, IGNORE or IGNORABLE declarations are inserted by B* according
-to the syntax of the variables bound; see below.  B* also supports multiple
-result expressions after the binding list; these are run in sequence and the
+to the syntax of the variables bound\; see below.  B* also supports multiple
+result expressions after the binding list\; these are run in sequence and the
 result of the last such form is returned.
 
 -- Binder Forms --
@@ -90,7 +94,10 @@ forms may be nested.
 
 (er a) produces an ER-LET* binding
 
-(list a b ...) produces a binding of (NTH 0 val), (NTH 1 val), etc, where val
+(list a b ...) produces a binding of (car val), (cadr val), etc, where val
+is the result of the corresponding expression
+
+(nths a b ...) produces a binding of (nth 0 val), (nth 1 val), etc, where val
 is the result of the corresponding expression
 
 (list* a b), `(,a . ,b) are alternatives to the CONS binder.
@@ -110,6 +117,13 @@ expands to something like this:
   (b* ((rest (of-bindings)))
     final-expr))
 ~ev[]
+These forms also create an \"implicit progn\" with multiple expressions, like
+this:
+~bv[]
+(b* (((if (atom a)) (cw \"a is an atom, returning 0\") 0)
+     ...)
+  ...)
+~ev[]
 
 -- Nesting Binders --
 The CONS, LIST, LIST*, and backtick binders may be nested arbitrarily inside
@@ -126,8 +140,9 @@ d bound to (cdr (mv-nth 1 <form>)).
 The following constructs may be used in place of variables:
 
 Dash (-), used as a top-level binding form, will run the corresponding
-expression for side-effects without binding its value.  Used as a lower-level
-binding form, it will cause the binding to be ignored or not created.  
+expressions (in an implicit progn) for side-effects without binding its value.
+Used as a lower-level binding form, it will cause the binding to be ignored or
+not created.
 
 Ampersand (&), used as a top-level binding form, will cause the corresponding
 expression to be ignored and not run at all.  Used as a lower-level binding
@@ -141,10 +156,10 @@ obtained by removing the ?, and will make an IGNORABLE declaration for this
 variable.
 
 -- User-Defined Binders --
-A new binder form may be created by defining a macro named PATBIND-<name>, in
-the ACL2 package.  We discuss the detailed interface of user-defined binders
-below.  First, DEF-PATBIND-MACRO provides a simple way to define certain user
-binders.  For example, this form is used to define the binder for CONS:
+A new binder form may be created by defining a macro named PATBIND-<name>.  We
+discuss the detailed interface of user-defined binders below.  First,
+DEF-PATBIND-MACRO provides a simple way to define certain user binders.  For
+example, this form is used to define the binder for CONS:
 (def-patbind-macro cons (car cdr))
 This defines a binder macro PATBIND-CONS which enables (cons a b) to be used as
 a binder form.  This binder form must take two arguments since two destructor
@@ -157,173 +172,58 @@ example, a binder produced by DEF-PATBIND-MACRO may only take a fixed number of
 arguments.  To more flexibly create binders, one must define binder macros by
 hand.
 
-A binder macro PATBIND-<NAME> must take four arguments ARGS, BINDING, IGNORES,
-and EXPR.  EXPR is the result expression to be run once the bindings are in
-place.  BINDING is the term to be decomposed and bound to ARGS, which are
-variables corresponding to the arguments given to the binder form.  Finally,
-IGNORES is a list of the same length as ARGS each element of which is either
-NIL or one of the symbols IGNORE (meaning the corresponding argument is an
-ignored variable) or IGNORABLE (meaning the corresponding argument is an
-ignorable variable.
+A binder macro PATBIND-<NAME> must take three arguments ARGS, BINDINGS,
+and EXPR.  The form
+~bv[]
+(b* (((binder arg1 arg2) binding1 binding2))
+   expr)
+~ev[]
+translates to a macro call
+~bv[]
+(patbind-binder (arg1 arg2) (binding1 binding2) expr).
+~ev[]
+That is, ARGS is the list of arguments given to the binder form, BINDINGS is
+the list of expressions bound to them, and EXPR is the result expression to be
+run once the bindings are in place.  The definition of the patbind-binder macro
+determines how this gets further expanded.  Some informative examples of these
+binder macros may be found in bstar.lisp\; simply search for macro declarations
+whose names begin with PATBIND-.  Here are some notes on defining binder macros.
 
-The binder macro must produce a form that performs the bindings of ARGS to the
-appropriate forms involving BINDING, makes declarations appropriate for
-IGNORES, and finally runs EXPR.  For examples of this, see the definitions of
-binder macros PATBIND-LIST and PATBIND-LIST*.
+Often the simplest way to accomplish the intended effect of a patbind macro is
+to have it construct another B* form to be recursively expanded, or to call
+other patbind macros.  See, for example, the definition of PATBIND-LIST.
 
-The default behavior on each binder is to first bind a variable to the result
-of computing the form.  When the form returns multiple values, this is the
-wrong behavior.  The MV and ER binders are treated specially for this purpose.
-User binders are treated this way if they end in the character +.
+Patbind macros for forms that are truly creating bindings should indeed use B*
+(or PATBIND, which is what B* expands to) to create these bindings, so that
+ignores and nestings are dealt with uniformly.  See, for example, the
+definition of PATBIND-NTHS.
+
+In order to get good performance, destructuring binders such as are produced by
+DEF-PATBIND-MACRO bind a variable to any binding that isn't already a variable
+or quoted constant.  This is important so that in the following form,
+~c[(foo x y)] is run only once:
+~bv[]
+(b* (((cons a b) (foo x y))) ...)
+~ev[]
+In these cases, it is good discipline to check the new variables introduced
+using the macro CHECK-VARS-NOT-FREE\; since ACL2 does not have gensym, this is
+the best option we have. See any definition produced by DEF-PATBIND-MACRO for
+examples, and additionally PATBIND-NTHS, PATBIND-ER, and so forth.
 ")
 
 
 
-;; Here are some examples of how it can be used:
-#||
-(b* ;; let*-like binding to a single variable:
-    ((x (cons 'a 'b))
-     ;; mv binding
-     ((mv y z) (return-two-values x x))
-     ;; No binding: expression evaluated for side effects
-     (- (cw "Hello")) ;; prints "Hello"
-     ;; Dont-care: expression not evaluated at all
-     ;; (why do we want this? see below.)
-     (& (cw "Hello")) ;; does not print "Hello"
-     ;; MV which ignores a value:
-     ((mv & a) (return-garbage-in-first-mv y z))
-     ;; Pattern-based binding using cons:
-     ((cons (cons b c) d) (must-return-nested-conses a))
-     ;; Alternate form of pattern binding with cons nests:
-     (`(,e (,f . ,g)) (makes-a-list-of-conses b))
-     ;; Pattern with user-defined constructor:
-     ((my-tuple foo bar hum) (something-of-type-my-tuple e c g))
-     ;; Don't-cares with pattern bindings:
-     ((my-tuple & (cons carbar &) hum) (something-else foo f hum))
-     ;; Pattern inside an mv:
-     ((mv a (cons & c)) (make-mv-with-cons)))
-  (some-expression ....))
-||#
-;; Syntax of b*:
-;; (b* <binder-list> <expr>) where
-;; 
-;; binder-list: ([(<pattern> <expr>)])
-;;
-;; pattern: <varname-symbol> | & | - | nil | (quote <expr>)
-;;          | (<pattern-constructor> [<pattern>])
-;;
-;; pattern-constructor: mv | cons | <user-defined-constructor>
-;;
-;;
-;; Pattern constructors can be defined using the macro
-;; def-patbind-macro, as in (def-patbind-macro cons (car cdr)), where
-;; the first argument is the constructor symbol and the second is a
-;; list of field accessor functions.
-
-
-
-
-;; Technical details:
-;;
-;; b* is based on another macro, patbind, much like let* is based on let;
-;; a call to b* expands to one or more nested calls to patbind.
-;; Specifically, as with let* and let, each item in the binder list
-;; results in one call to patbind, so that variables bound in the list
-;; are available for use in the next binding expression.
-;;
-;; Each binding is specified by a pattern and an expression.  The
-;; expression is evaluated and the pattern is then matched against its
-;; value recursively, splitting into the following cases:
-;;
-;; Pattern is a variable symbol:  the variable is simply bound to the
-;; expression using let.
-;;
-;; Pattern is the - wildcard:  The expression is evaluated for side
-;; effects and not bound.
-;;
-;; Pattern is the & wildcard, a quoted constant, or the symbol nil or
-;; t:  The binding is ignored and the expression is never evaluated.
-;;
-;; Otherwise, the pattern must be a constructor expression, a cons
-;; where the car is a symbol with associated macro named
-;; patbind-<symbol>, and the cdr is a list of patterns.  The cdr, or
-;; argument list, is processed as follows to produce a variable list
-;; and an ignore list, as follows.
-;;
-;; - Each variable symbol is added to the variable list.
-;;
-;; - Each wildcard, boolean symbol, and quoted constant has a variable
-;; name created for it which is added to the variable and ignore lists.
-;;
-;; - Each constructor call has a variable name created for it which is
-;; added to the variable list.
-;;
-;; The inner expression is then augmented with surrounding calls to
-;; patbind for each pair (pattern, variable) from the argument list and
-;; the variable list.  This expression is passed, along with the
-;; variable list, assigned expression, and ignore list, to the macro
-;; patbind-<symbol>, which is user-defined.  In sane cases, the action of the
-;; macro is to surround the augmented inner expression with a binding
-;; for each of the variables in the variable list.
-;; 
-;; Here are some examples of how patbind expands:
-;; (patbind (cons a (cons & b)) (some-function-call) (the-answer))
-;; Since the pattern (cons a (cons & b)) is a constructor call and the
-;; assigned expression is not evaluated, we first bind its result to a
-;; variable.  The variable name chosen is the pattern itself read into
-;; a symbol, which we would not expect to conflict with any other
-;; variable name.
-;; (let ((|(CONS A (CONS & B))| (some-function-call)))
-;;   (patbind (cons a (cons & b)) |(CONS A (CONS & B))| (the-answer)))
-;; The inner patbind has its assigned expression already evaluated, and
-;; its pattern is a constructor call; the constructor is CONS and the
-;; argument list is (A (CONS & B)).  The variable list for this is (A
-;; |(CONS & B)|) and the ignore list is empty.  The inner expression
-;; is augmented by binding the patterns to the variables, although
-;; binding a to itself is skipped:
-;; (patbind (cons & b) |(CONS & B)| (the-answer))
-;; and this augmented inner expression is passed to the PATBIND-CONS
-;; macro with the variable list, assigned expression, and ignore list:
-;; (patbind-cons (a |(CONS & B)|) |(CONS A (CONS & B))| nil
-;;   (patbind (cons & b) |(CONS & B)| (the-answer)))
-;; The patbind-cons macro forms a let expression binding the first
-;; variable in the list to the car of the assigned expression and the
-;; second to the cdr:
-;; (let ((a (car |(CONS A (CONS & B))|))
-;;       (|(CONS & B)| (cdr |(CONS A (CONS & B))|)))
-;;   (patbind (cons & b) |(CONS & B)| (the-answer)))
-;; The inner patbind also has a cons constructor call as its pattern
-;; which is processed as follows: The argument list is (& b), so the
-;; variable list is (ignore-0 b) and the ignore list is (ignore-0).
-;; The augmented inner expression is
-;; (patbind & ignore-0 (the-answer))
-;; and the patbind-cons call is
-;; (patbind-cons (ignore-0 b) |(CONS & B)| (ignore-0)
-;;   (patbind & ignore-0 (the-answer)))
-;; The patbind-cons macro simply removes variables in the ignore list
-;; from its let binding, so the result of this expansion is
-;; (let ((b (cdr |(CONS & B)|)))
-;;   (patbind & ignore-0 (the-answer)))
-;; The inner patbind call has the wildcard symbol & as its pattern, so it
-;; ignores the binding altogether and expands to (the-answer).
-;; So the full expansion is equivalent to
-;; (let ((|(CONS A (CONS & B))| (some-function-call)))
-;;   (let ((a (car |(CONS A (CONS & B))|))
-;;         (|(CONS & B)| (cdr |(CONS A (CONS & B))|)))
-;;     (let ((b (cdr |(CONS & B)|)))
-;;       (the-answer)))).
-
-
-
-
-
 (include-book "pack")
+(include-book "progndollar")
 
-(defun patbind-macro-name (binder)
-  (intern (concatenate 'string
-                       "PATBIND-"
-                       (symbol-name binder))
-          "ACL2"))
+(defun macro-name-for-patbind (binder)
+  (intern-in-package-of-symbol
+   (concatenate 'string
+                "PATBIND-"
+                (symbol-name binder))
+   (if (equal (symbol-package-name binder) "COMMON-LISP")
+       'acl2::foo
+     binder)))
 
 (defconst *patbind-special-syms* '(t nil & -))
 
@@ -337,29 +237,25 @@ User binders are treated this way if they end in the character +.
   (str-num-sym "IGNORE-" n))
 
 
-
-(verify-termination doubleton-list-p)
-(verify-guards doubleton-list-p)
-
-
-(defun debuggable-doubleton-list-p (x)
+(defun debuggable-binder-list-p (x)
   (declare (xargs :guard t))
-  (mbe :logic (doubleton-list-p x)
-       :exec (cond ((atom x) 
-                    (or (equal x nil)
-                        (cw "; Not a doubleton-list-p: ends with ~x0, instead of nil.~%" x)))
-                   ((and (true-listp (car x))
-                         (eql (length (car x)) 2))
-                    (debuggable-doubleton-list-p (cdr x)))
-                   (t
-                    (cw "; Not a doubleton-list-p: first bad entry is ~x0.~%" (car x))))))
+  (cond ((atom x) 
+         (or (equal x nil)
+             (cw "; Not a binder list; ends with ~x0, instead of nil.~%" x)))
+        ((and (consp (car x))
+              (consp (cdar x))
+              (true-listp (cddar x)))
+         (debuggable-binder-list-p (cdr x)))
+        (t
+         (cw "; Not a binder list; first bad entry is ~x0.~%" (car x)))))
 
-(defun patbind-decode-varname (pattern)
+(defun decode-varname-for-patbind (pattern)
   (let* ((name (symbol-name pattern))
-         (?p (and (<= 1 (length name))
+         (len (length name))
+         (?p (and (<= 1 len)
                   (eql (char name 0) #\?)))
          (?!p (and ?p
-                   (<= 2 (length name))
+                   (<= 2 len)
                    (eql (char name 1) #\!)))
          (sym (cond 
                (?!p (intern-in-package-of-symbol
@@ -372,384 +268,400 @@ User binders are treated this way if they end in the character +.
                    (?p 'ignorable))))
     (mv sym ignorep)))
 
-(defun patbind-nest (args vars expr)
-  (if (atom args)
-      expr
-    (if (atom (car args))
-        (patbind-nest (cdr args) (cdr vars) expr)
-      `(patbind ,(car args) ,(car vars)
-                ,(patbind-nest (cdr args) (cdr vars) expr)))))
 
 
-(defun patbind-find-ignores (ignore-or-ignorable vars ignores acc)
-  (if (atom vars)
-      acc
-    (patbind-find-ignores
-     ignore-or-ignorable
-     (cdr vars) (cdr ignores)
-     (if (eq ignore-or-ignorable (car ignores))
-         (cons (car vars) acc)
-       acc))))
-
-(defun patbind-var-ignore-list (args vars igcount ignores)
-  (if (atom args)
-      (mv (reverse vars) (reverse ignores))
-    (mv-let (sym ignorep)
-      (cond ((or (member (car args) *patbind-special-syms*)
-                 (quotep (car args))
-                 (and (atom (car args)) (not (symbolp (car args)))))
-             (let ((var (ignore-var-name igcount)))
-               (mv var 'ignore)))
-            ((symbolp (car args))
-             (patbind-decode-varname (car args)))
-            (t (mv (pack (car args)) nil)))
-      (patbind-var-ignore-list (cdr args) (cons sym vars)
-                               (if (eql ignorep 'ignore)
-                                   (1+ igcount)
-                                 igcount)
-                               (cons ignorep ignores)))))
-
-
-
-(defun patbindfn (pattern assign-expr nested-expr)
-  (cond ((and (consp assign-expr) (not (eq (car assign-expr) 'quote))
-              (consp pattern)
-              (not (member (car pattern) '(mv er when unless if)))
-              (not (and (symbolp (car pattern))
-                        (let ((str (symbol-name (car pattern))))
-                          (and (not (equal str ""))
-                               (eql (char str (1- (length str))) #\+))))))
-         (let ((var (pack pattern)))
-           `(let ((,var ,assign-expr))
-              (patbind ,pattern ,var ,nested-expr))))
-        ((eq pattern '-)
-         `(prog2$ ,assign-expr
+(defun patbindfn (pattern assign-exprs nested-expr)
+  (cond ((eq pattern '-)
+         ;; A dash means "run this for side effects."  In this case we allow
+         ;; multiple terms; these form an implicit progn, in the common-lisp sense.
+         `(prog2$ (progn$ . ,assign-exprs)
                   ,nested-expr))
         ((member pattern *patbind-special-syms*)
+         ;; &, T, NIL mean "don't bother evaluating this."
          nested-expr)
         ((atom pattern)
-         (mv-let (sym ignorep)
-           (patbind-decode-varname pattern)
-           `(let ((,sym ,assign-expr))
-              ,@(and ignorep `((declare (,ignorep ,sym))))
-              ,nested-expr)))
+         ;; A binding to a single variable.  Here we don't allow multiple
+         ;; expressions; we believe it's more readable to use - to run things
+         ;; for side effects, and this might catch some paren errors.
+         (if (cdr assign-exprs)
+             (er hard 'b* "~
+The B* binding of ~x0 to ~x1 isn't allowed because the binding of a variable must be a
+single term." pattern assign-exprs)
+           (mv-let (sym ignorep)
+             (decode-varname-for-patbind pattern)
+             ;; Can we just refuse to bind a variable marked ignored?
+             (if (eq ignorep 'ignore)
+                 nested-expr
+               `(let ((,sym ,(car assign-exprs)))
+                  ,@(and ignorep `((declare (,ignorep ,sym))))
+                  ,nested-expr)))))
         ((eq (car pattern) 'quote)
+         ;; same idea as &, t, nil
          nested-expr)
-        ((member (car pattern) '(when unless if))
+        (t ;; Binding macro call.
          (let* ((binder (car pattern))
-                (patbind-macro (patbind-macro-name binder))
+                (patbind-macro (macro-name-for-patbind binder))
                 (args (cdr pattern)))
-           `(,patbind-macro ,args ,assign-expr nil
-                            ,nested-expr)))
-        (t (let* ((binder (car pattern))
-                  (patbind-macro (patbind-macro-name binder))
-                  (args (cdr pattern)))
-             (mv-let 
-              (vars ignores)
-              (patbind-var-ignore-list args nil 0 nil)
-              `(,patbind-macro ,vars ,assign-expr ,ignores
-                               ,(patbind-nest args vars nested-expr)))))))
+           `(,patbind-macro ,args ,assign-exprs ,nested-expr)))))
              
         
 
-(defun mk-prog2$-nest (exprs)
-  (declare (xargs :guard (consp exprs)))
-  (if (atom (cdr exprs))
-      (car exprs)
-    `(prog2$ ,(car exprs)
-             ,(mk-prog2$-nest (cdr exprs)))))
          
          
-(defmacro patbind (pattern assign-expr nested-expr)
-  (patbindfn pattern assign-expr nested-expr))
+(defmacro patbind (pattern assign-exprs nested-expr)
+  (patbindfn pattern assign-exprs nested-expr))
 
 
 (defun b*-fn1 (bindlist expr)
-  (declare (xargs :guard (debuggable-doubleton-list-p bindlist)))
+  (declare (xargs :guard (debuggable-binder-list-p bindlist)))
   (if (atom bindlist)
       expr
-    `(patbind ,(caar bindlist) ,(cadar bindlist)
+    `(patbind ,(caar bindlist) ,(cdar bindlist)
               ,(b*-fn1 (cdr bindlist) expr))))
 
 (defun b*-fn (bindlist exprs)
-  (declare (xargs :guard (and (debuggable-doubleton-list-p bindlist)
+  (declare (xargs :guard (and (debuggable-binder-list-p bindlist)
                               (consp exprs))))
-  (b*-fn1 bindlist (mk-prog2$-nest exprs)))
+  (b*-fn1 bindlist `(progn$ . ,exprs)))
 
 (defmacro b* (bindlist expr &rest exprs)
-  (declare (xargs :guard (debuggable-doubleton-list-p bindlist)))
+  (declare (xargs :guard (debuggable-binder-list-p bindlist)))
   (b*-fn bindlist (cons expr exprs)))
 
 
 
 
-(defun binding-list (args bindings ignores)
+
+(defmacro destructure-guard (binder args bindings len)
+  `(and (or (and (true-listp ,args)
+                 . ,(and len `((= (length ,args) ,len))))
+            (cw "~%~%**** ERROR ****
+Pattern constructor ~x0 needs a true-list of ~@1arguments, but was given ~x2~%~%"
+                ',binder ,(if len `(msg "~x0 " ,len) "")
+                ,args))
+        (or (and (consp ,bindings)
+                 (eq (cdr ,bindings) nil))
+            (cw "~%~%**** ERROR ****
+Pattern constructor ~x0 needs exactly one binding expression, but was given ~x1~%~%"
+                ',binder ,bindings))))
+
+
+
+(defun destructor-binding-list (args destructors binding)
   (if (atom args)
       nil
-    (if (eql (car ignores) 'ignore)
-        (binding-list (cdr args) (cdr bindings) (cdr ignores))
-      (cons (list (car args) (car bindings))
-            (binding-list (cdr args) (cdr bindings) (cdr ignores))))))
-
-
-(defun destructor-binding-list (destructors)
-  (if (atom destructors)
-      nil
-    ``((,',(car destructors) ,binding) .
-       ,,(destructor-binding-list (cdr destructors)))))
+    (cons (list (car args) (list (car destructors) binding))
+          (destructor-binding-list (cdr args) (cdr destructors) binding))))
 
 (defmacro def-patbind-macro (binder destructors)
-  (let ((binding-list (destructor-binding-list destructors))
-        (len (length destructors)))
-  `(defmacro ,(patbind-macro-name binder) (args binding ignores expr)
-     (declare (xargs :guard (and (true-listp args)
-                                 (= (length args) ,len))))
-     (let ((ignorable (patbind-find-ignores 'ignorable args ignores nil)))
-     `(let ,(binding-list args ,binding-list ignores)
-        ,@(and ignorable `((declare (ignorable . ,ignorable))))
-        ,expr)))))
+  (let ((len (length destructors)))
+    `(defmacro ,(macro-name-for-patbind binder) (args bindings expr)
+       (declare (xargs :guard
+                       (destructure-guard ,binder args bindings ,len)))
+       (let* ((binding (car bindings))
+              (computedp (or (atom binding)
+                             (eq (car binding) 'quote)))
+              (bexpr (if computedp binding (pack binding)))
+              (binders (destructor-binding-list args ',destructors bexpr)))
+         (if computedp
+             `(b* ,binders ,expr)
+           `(let ((,bexpr ,binding))
+              (b* ,binders
+                (check-vars-not-free (,bexpr) ,expr))))))))
+
+;; The arg might be a plain variable, an ignored or ignorable variable, or a
+;; binding expression.
+(defun var-ignore-list-for-patbind-mv (args igcount mv-vars binders ignores ignorables freshvars)
+  (if (atom args)
+      (mv (reverse mv-vars)
+          (reverse binders)
+          (reverse ignores)
+          (reverse ignorables)
+          (reverse freshvars))
+    (mv-let (mv-var binder freshp ignorep)
+      (cond ((or (member (car args) *patbind-special-syms*)
+                 (quotep (car args))
+                 (and (atom (car args)) (not (symbolp (car args)))))
+             (let ((var (ignore-var-name igcount)))
+               (mv var nil nil 'ignore)))
+            ((symbolp (car args))
+             (mv-let (sym ignorep)
+               (decode-varname-for-patbind (car args))
+               (case ignorep
+                 (ignore (mv sym nil nil 'ignore))
+                 (ignorable (mv sym nil nil 'ignorable))
+                 (t (mv sym nil nil nil)))))
+            (t ;; (and (consp (car args))
+             ;;                   (not (eq (caar args) 'quote)))
+             (let ((var (pack (car args))))
+               (mv var (list (car args) var) t nil))))
+      (var-ignore-list-for-patbind-mv
+       (cdr args)
+       (if (eq ignorep 'ignore) (1+ igcount) igcount)
+       (cons mv-var mv-vars)
+       (if binder (cons binder binders) binders)
+       (if (eq ignorep 'ignore) (cons mv-var ignores) ignores)
+       (if (eq ignorep 'ignorable) (cons mv-var ignorables) ignorables)
+       (if freshp (cons mv-var freshvars) freshvars)))))
+          
 
 
-
-(defmacro patbind-mv (args binding ignores expr)
-  (let ((ignore (patbind-find-ignores 'ignore args ignores nil))
-        (ignorable (patbind-find-ignores 'ignorable args ignores nil)))
-    `(mv-let ,args ,binding 
-       ,@(and (or ignore ignorable)
-              `((declare ,@(and ignore `((ignore . ,ignore)))
-                         . ,(and ignorable `((ignorable . ,ignorable))))))
-       ,expr)))
+(defmacro patbind-mv (args bindings expr)
+  (declare (xargs :guard (destructure-guard mv args bindings nil)))
+  (mv-let (vars binders ignores ignorables freshvars)
+    (var-ignore-list-for-patbind-mv args 0 nil nil nil nil nil)
+    `(mv-let ,vars ,(car bindings)
+       (declare (ignore . ,ignores))
+       (declare (ignorable . ,ignorables))
+       (check-vars-not-free
+        ,ignores
+        (b* ,binders
+          (check-vars-not-free ,freshvars ,expr))))))
 
 (def-patbind-macro cons (car cdr))
 
-(defun list-binding-list (args n form ignores)
+(defun nths-binding-list (args n form)
   (if (atom args)
       nil
-    (if (eql (car ignores) 'ignore)
-        (list-binding-list (cdr args) (1+ n) form (cdr ignores))
-      (cons (list (car args) `(nth ,n ,form))
-            (list-binding-list (cdr args) (1+ n) form (cdr ignores))))))
+    (cons (list (car args) `(nth ,n ,form))
+          (nths-binding-list (cdr args) (1+ n) form))))
 
 
-(defun list*-binding-list (args form ignores)
-  (if (atom (cdr args))
-      (if (eql (car ignores) 'ignore)
-          nil
-        (list (list (car args) form)))
-    (if (eql (car ignores) 'ignore)
-        (list*-binding-list (cdr args) `(cdr ,form) (cdr ignores))
-      (cons (list (car args) `(car ,form))
-            (list*-binding-list (cdr args) `(cdr ,form) (cdr ignores))))))
-
-
-(defmacro patbind-list (args binding ignores expr)
-  (declare (xargs :guard (true-listp args)))
-  (let ((ignorable (patbind-find-ignores 'ignorable args ignores nil)))
-    `(let ,(list-binding-list args 0 binding ignores)
-       ,@(and ignorable `((declare (ignorable . ,ignorable))))
-       ,expr)))
-
-
-(defmacro patbind-list* (args binding ignores expr)
-  (declare (xargs :guard (true-listp args)))
-  (let ((ignorable (patbind-find-ignores 'ignorable args ignores nil)))
-    `(let ,(list*-binding-list args binding ignores)
-       ,@(and ignorable `((declare (ignorable . ,ignorable))))
-       ,expr)))
-
-(defmacro patbind-er (args binding ignores expr)
-  (declare (xargs :guard (and (consp args) (eq (cdr args) nil))))
-  (case (car ignores)
-    (ignore `(er-progn ,binding ,expr))
-    (ignorable `(er-let* ((,(car args) ,binding))
-                         (let ((,(car args) ,(car args)))
-                           (declare (ignorable ,(car args)))
-                         ,expr)))
-    (otherwise `(er-let* ((,(car args) ,binding))
-                         ,expr))))
-
-(defmacro patbind-state-global (args binding ignores expr)
-  (declare (ignorable ignores))
-  `(state-global-let*
-    ((,(car args) ,binding))
-    ,expr))
-
-
-(defmacro patbind-when (args bindings ignores expr)
-  (declare (ignore ignores)
-           (xargs :guard (and (consp args) (eq (cdr args) nil))))
-  `(if ,(car args)
-       ,bindings
-     ,expr))
-
-(defmacro patbind-if (args bindings ignores expr)
-  (declare (ignore ignores)
-           (xargs :guard (and (consp args) (eq (cdr args) nil))))
-  `(if ,(car args)
-       ,bindings
-     ,expr))
-
-(defmacro patbind-unless (args bindings ignores expr)
-  (declare (ignore ignores)
-           (xargs :guard (and (consp args) (eq (cdr args) nil))))
-  `(if ,(car args)
-       ,expr
-     ,bindings))
+(defmacro patbind-nths (args bindings expr)
+  (declare (xargs :guard (destructure-guard nths args bindings nil)))
+  (let* ((binding (car bindings))
+         (evaledp (or (atom binding) (eq (car binding) 'quote)))
+         (form (if evaledp binding (pack binding)))
+         (binders (nths-binding-list args 0 form)))
+    (if evaledp
+        `(b* ,binders ,expr)
+      `(let ((,form ,binding))
+         (b* ,binders
+           (check-vars-not-free (,form) ,expr))))))
   
 
 
-(local
- (progn
-   (defmacro transl-equal (x y)
-     `(mv-let (flgx valx bindings state)
-        (translate1 ,x :stobjs-out
-                    '((:stobjs-out . :stobjs-out))
-                    t :top-level (w state) state)
-        (declare (ignore bindings))
-        (mv-let (flgy valy bindings state)
-          (translate1 ,y :stobjs-out
-                      '((:stobjs-out . :stobjs-out))
-                      t :top-level (w state) state)
-          (declare (ignore bindings))
-          (mv (and flgx flgy) (equal valx valy) state))))
 
 
-   (defun return-two-values (a b)
-     (mv a b))
+(defmacro patbind-list (args bindings expr)
+  (declare (xargs :guard (destructure-guard list args bindings nil)))
+  (if (atom args)
+      expr
+    `(patbind-cons (,(car args) (list . ,(cdr args))) ,bindings ,expr)))
 
-   (defun transl-equal-tests-fn (tests)
-     (if (atom tests)
-         `(mv nil state)
-       `(mv-let (err val state)
-          (transl-equal ',(caar tests) ',(cadar tests))
-          (if (or err (not val))
-              (mv ',(car tests) state)
-            ,(transl-equal-tests-fn (cdr tests))))))
+(defmacro patbind-list* (args bindings expr)
+  (declare (xargs :guard (and (consp args)
+                              (destructure-guard list* args bindings nil))))
+  (if (atom (cdr args))
+      `(patbind ,(car args) ,bindings ,expr)
+    `(patbind-cons (,(car args) (list* . ,(cdr args))) ,bindings ,expr)))
 
-   (defmacro transl-equal-tests (&rest tests)
-     (transl-equal-tests-fn tests))
+(defmacro patbind-er (args bindings expr)
+  (declare (xargs :guard (destructure-guard er args bindings 1)))
+  `(mv-let (patbind-er-fresh-variable-for-erp
+            patbind-er-fresh-variable-for-val
+            state)
+     ,(car bindings)
+     (if patbind-er-fresh-variable-for-erp
+         (mv patbind-er-fresh-variable-for-erp
+             patbind-er-fresh-variable-for-val
+             state)
+       (patbind ,(car args)
+                (patbind-er-fresh-variable-for-val)
+                (check-vars-not-free
+                 (patbind-er-fresh-variable-for-val
+                  patbind-er-fresh-variable-for-erp)
+                 ,expr)))))
 
-
-   (defmacro patbind-run-tests (&rest tests)
-     `(make-event
-       (mv-let (err state)
-         (transl-equal-tests ,@tests)
-         (if err
-             (mv t
-                 (er hard? 'patbind-run-tests
-                     "~% ****** ERROR ******~%~
-Testing of the patbind macro failed on expression ~x0~%~%" err)
-                 state)
-           (value (prog2$ (cw "
-Testing of the patbind macro passed.~%")
-                          `(value-triple 'tests-ok)))))
-       :check-expansion (value-triple 'tests-ok)))
-
-
-   (patbind-run-tests
-;; TEST CASES
-
-    ((patbind (cons (cons a b) c) x (list a b c))
-     (let ((|(CONS A B)| (car x))
-           (c (cdr x)))
-       (let ((a (car |(CONS A B)|))
-             (b (cdr |(CONS A B)|)))
-         (list a b c))))
-
-    ((patbind x (cons 'a 'b) x)
-     (let ((x (cons 'a 'b))) x))
-
-    ((patbind (mv a b) (mv 'a 'b) (list a b))
-     (mv-let (a b) (mv 'a 'b) (list a b)))
-
-    ((patbind & (cw "Hello") nil)
-     nil)
-
-    ((patbind - (cw "Hello") nil)
-     (prog2$ (cw "Hello")
-             nil))
-
-    ((patbind (cons a &) '(a b) a)
-     (let ((a (car '(a b))))
-       a))
-
-    ((patbind (cons (cons a b) c) x
-              (list a b c))
-     (let ((|(CONS A B)| (car x))
-           (c (cdr x)))
-       (let ((a (car |(CONS A B)|))
-             (b (cdr |(CONS A B)|)))
-         (list a b c))))
-
-    ((patbind (cons (cons a b) c) (cons x y)
-              (list a b c))
-     (let ((|(CONS (CONS A B) C)| (cons x y)))
-       (let ((|(CONS A B)| (car |(CONS (CONS A B) C)|))
-             (c (cdr |(CONS (CONS A B) C)|)))
-         (let ((a (car |(CONS A B)|))
-               (b (cdr |(CONS A B)|)))
-           (list a b c)))))
-
-    ((patbind (cons (cons & b) c) (cons x y)
-              (list b c))
-     (let ((|(CONS (CONS & B) C)| (cons x y)))
-       (let ((|(CONS & B)| (car |(CONS (CONS & B) C)|))
-             (c (cdr |(CONS (CONS & B) C)|)))
-         (let ((b (cdr |(CONS & B)|)))
-           (list b c)))))
-
-    ((patbind (cons (cons a &) c) (cons x y)
-              (list a c))
-     (let ((|(CONS (CONS A &) C)| (cons x y)))
-       (let ((|(CONS A &)| (car |(CONS (CONS A &) C)|))
-             (c (cdr |(CONS (CONS A &) C)|)))
-         (let ((a (car |(CONS A &)|)))
-           (list a c)))))
+(defmacro patbind-state-global (args bindings expr)
+  (declare (xargs :guard
+                  (and (destructure-guard
+                        state-global args bindings 1)
+                       (or (symbolp (car args))
+                           (cw "~%~%**** ERROR ****
+Pattern constructor ~x0 needs a single argument which is a symbol, but got ~x1~%~%"
+                               'state-global args)))))
+  `(state-global-let*
+    ((,(car args) ,(car bindings)))
+    ,expr))
 
 
-    ((patbind (mv (cons a (cons b c)) d)
-              (return-two-values x y)
-              (list a b c d))
-     (mv-let (|(CONS A (CONS B C))| d)
-       (return-two-values x y)
-       (let ((a (car |(CONS A (CONS B C))|))
-             (|(CONS B C)| 
-              (cdr |(CONS A (CONS B C))|)))
-         (let ((b (car |(CONS B C)|))
-               (c (cdr |(CONS B C)|)))
-           (list a b c d)))))
+(defmacro patbind-when (args bindings expr)
+  (declare (xargs :guard (and (consp args) (eq (cdr args) nil))))
+  `(if ,(car args)
+       (progn$ . , bindings)
+     ,expr))
 
-    ((patbind (mv (cons a (cons b c)) &)
-              (return-two-values x y)
-              (list a b c d))
-     (mv-let (|(CONS A (CONS B C))| ignore-0)
-       (return-two-values x y)
-       (declare (ignore ignore-0))
-       (let ((a (car |(CONS A (CONS B C))|))
-             (|(CONS B C)| 
-              (cdr |(CONS A (CONS B C))|)))
-         (let ((b (car |(CONS B C)|))
-               (c (cdr |(CONS B C)|)))
-           (list a b c d)))))
+(defmacro patbind-if (args bindings expr)
+  (declare (xargs :guard (and (consp args) (eq (cdr args) nil))))
+  `(if ,(car args)
+       (progn$ . ,bindings)
+     ,expr))
 
-    ((patbind (mv (cons a (cons & c)) &)
-              (return-two-values x y)
-              (list a c d))
-     (mv-let (|(CONS A (CONS & C))| ignore-0)
-       (return-two-values x y)
-       (declare (ignore ignore-0))
-       (let ((a (car |(CONS A (CONS & C))|))
-             (|(CONS & C)| 
-              (cdr |(CONS A (CONS & C))|)))
-         (let ((c (cdr |(CONS & C)|)))
-           (list a c d)))))
+(defmacro patbind-unless (args bindings expr)
+  (declare (xargs :guard (and (consp args) (eq (cdr args) nil))))
+  `(if ,(car args)
+       ,expr
+     (progn$ . ,bindings)))
+  
+
+(set-state-ok t)
+
+(with-output 
+ :off warning
+ (local
+  (progn
+    (defun return-two-values (a b)
+      (mv a b))
+
+    (defun transl-equal-tests-fn (tests)
+      (if (atom tests)
+          `(mv nil state)
+        `(mv-let (err val state)
+           (transl-equal ',(caar tests) ',(cadar tests))
+           (if (or err (not val))
+               (mv ',(car tests) state)
+             ,(transl-equal-tests-fn (cdr tests))))))
+
+    (defmacro transl-equal-tests (&rest tests)
+      (transl-equal-tests-fn tests))
+
+
+    (defun patbind-tests-fn (tests state)
+      (declare (xargs :mode :program))
+      (if (atom tests)
+          (value '(value-triple :invisible))
+        (mv-let (erp val state)
+          (thm-fn `(equal ,(caar tests) ,(cadar tests))
+                  state '(("goal" :in-theory nil)) nil nil)
+          (if erp
+              (mv (msg "~% ****** ERROR ******~%~
+Testing of the patbind macro failed on expression ~x0~%~%" (car tests))
+                  val state)
+            (patbind-tests-fn (cdr tests) state)))))
+
+    (defmacro patbind-run-tests (&rest tests)
+      `(make-event
+        (patbind-tests-fn ',tests state)))
+    ;;        (mv-let (err val state)
+    ;;          (transl-equal-tests ,@tests)
+    ;;          (declare (ignore val))
+    ;;          (if err
+    ;;              (mv t
+    ;;                  (er hard? 'patbind-run-tests
+    ;;                      "~% ****** ERROR ******~%~
+    ;; Testing of the patbind macro failed on expression ~x0~%~%" err)
+    ;;                  state)
+    ;;            (value (prog2$ (cw "
+    ;; Testing of the patbind macro passed.~%")
+    ;;                           `(value-triple 'tests-ok)))))
+    ;;        :check-expansion (value-triple 'tests-ok)))
+
+
+    (patbind-run-tests
+     ;; TEST CASES
+
+     ((patbind (cons (cons a b) c) (x) (list a b c))
+      (let* ((|(CAR X)| (car x))
+             (c (cdr x)))
+        (let* ((a (car |(CAR X)|))
+               (b (cdr |(CAR X)|)))
+          (list a b c))))
+
+     ((patbind x ((cons 'a 'b)) x)
+      (let ((x (cons 'a 'b))) x))
+
+     ((patbind (mv a b) ((mv 'a 'b)) (list a b))
+      (mv-let (a b) (mv 'a 'b) (list a b)))
+
+     ((patbind & ((cw "Hello")) nil)
+      nil)
+
+     ((patbind - ((cw "Hello")) nil)
+      (prog2$ (cw "Hello")
+              nil))
+
+     ((patbind (cons a &) ('(a b)) a)
+      (let ((a (car '(a b))))
+        a))
+
+     ((patbind (cons (cons a b) c) (x)
+               (list a b c))
+      (let ((|(CONS A B)| (car x))
+            (c (cdr x)))
+        (let ((a (car |(CONS A B)|))
+              (b (cdr |(CONS A B)|)))
+          (list a b c))))
+
+     ((patbind (cons (cons a b) c) ((cons x y))
+               (list a b c))
+      (let ((|(CONS (CONS A B) C)| (cons x y)))
+        (let ((|(CONS A B)| (car |(CONS (CONS A B) C)|))
+              (c (cdr |(CONS (CONS A B) C)|)))
+          (let ((a (car |(CONS A B)|))
+                (b (cdr |(CONS A B)|)))
+            (list a b c)))))
+
+     ((patbind (cons (cons & b) c) ((cons x y))
+               (list b c))
+      (let ((|(CONS (CONS & B) C)| (cons x y)))
+        (let ((|(CONS & B)| (car |(CONS (CONS & B) C)|))
+              (c (cdr |(CONS (CONS & B) C)|)))
+          (let ((b (cdr |(CONS & B)|)))
+            (list b c)))))
+
+     ((patbind (cons (cons a &) c) ((cons x y))
+               (list a c))
+      (let ((|(CONS (CONS A &) C)| (cons x y)))
+        (let ((|(CONS A &)| (car |(CONS (CONS A &) C)|))
+              (c (cdr |(CONS (CONS A &) C)|)))
+          (let ((a (car |(CONS A &)|)))
+            (list a c)))))
+
+
+     ((patbind (mv (cons a (cons b c)) d)
+               ((return-two-values x y))
+               (list a b c d))
+      (mv-let (|(CONS A (CONS B C))| d)
+        (return-two-values x y)
+        (let ((a (car |(CONS A (CONS B C))|))
+              (|(CONS B C)| 
+               (cdr |(CONS A (CONS B C))|)))
+          (let ((b (car |(CONS B C)|))
+                (c (cdr |(CONS B C)|)))
+            (list a b c d)))))
+
+     ((patbind (mv (cons a (cons b c)) &)
+               ((return-two-values x y))
+               (list a b c d))
+      (mv-let (|(CONS A (CONS B C))| ignore-0)
+        (return-two-values x y)
+        (declare (ignore ignore-0))
+        (let ((a (car |(CONS A (CONS B C))|))
+              (|(CONS B C)| 
+               (cdr |(CONS A (CONS B C))|)))
+          (let ((b (car |(CONS B C)|))
+                (c (cdr |(CONS B C)|)))
+            (list a b c d)))))
+
+     ((patbind (mv (cons a (cons & c)) &)
+               ((return-two-values x y))
+               (list a c d))
+      (mv-let (|(CONS A (CONS & C))| ignore-0)
+        (return-two-values x y)
+        (declare (ignore ignore-0))
+        (let ((a (car |(CONS A (CONS & C))|))
+              (|(CONS & C)| 
+               (cdr |(CONS A (CONS & C))|)))
+          (let ((c (cdr |(CONS & C)|)))
+            (list a c d)))))
  
-    ((patbind `(,a ,b) (cons x y) (list a b))
-     (let ((|(CONS A (CONS B (QUOTE NIL)))| (cons x y)))
-       (let ((a (car |(CONS A (CONS B (QUOTE NIL)))|))
-             (|(CONS B (QUOTE NIL))|
-              (cdr |(CONS A (CONS B (QUOTE NIL)))|)))
-         (let ((b (car |(CONS B (QUOTE NIL))|)))
-           (list a b)))))
+     ((patbind `(,a ,b) ((cons x y)) (list a b))
+      (let ((|(CONS A (CONS B (QUOTE NIL)))| (cons x y)))
+        (let ((a (car |(CONS A (CONS B (QUOTE NIL)))|))
+              (|(CONS B (QUOTE NIL))|
+               (cdr |(CONS A (CONS B (QUOTE NIL)))|)))
+          (let ((b (car |(CONS B (QUOTE NIL))|)))
+            (list a b)))))
 
-    )))
+     ))))
